backend/RTLLSim.v
@@ -54,7 +54,26 @@ Record mrelT_propsT (t:Type) (ops:mrelT_opsT t): Prop := mkmrelT_propsT {
            (H1: initial_state p1 s1)
            (H2: initial_state p2 s2),
     exists mrel_init i_init,
-      ops.(sem) mrel_init p1 p2 i_init s1 s2
+      ops.(sem) mrel_init p1 p2 i_init s1 s2;
+  Hexternal_call:
+    forall p1 p2 s1 s2 cs1 cs2 ef args1 args2 m1 m2 evt s1' res1 m1' mrel i
+           (Hp: program_weak_lsim
+                  (@common_fundef_dec _) fn_sig
+                  (@common_fundef_dec _) fn_sig
+                  (@Errors.OK _)
+                  p1 p2)
+           (Hs1: s1 = Callstate cs1 (External ef) args1 m1)
+           (Hs2: s2 = Callstate cs2 (External ef) args2 m2)
+           (Hs1': s1' = Returnstate cs1 res1 m1')
+           (Hmrel: ops.(sem) mrel p1 p2 i s1 s2)
+           (Hs2: step (Genv.globalenv p1) s1 evt s1')
+           (Hargs: list_forall2 (ops.(sem_value) mrel) args1 args2),
+    exists mrel' i' s2' res2 m2',
+      s2' = Returnstate cs2 res2 m2' /\
+      step (Genv.globalenv p2) s2 evt s2' /\
+      ops.(sem) mrel' p1 p2 i' s1' s2' /\
+      ops.(sem_value) mrel' res1 res2 /\
+      ops.(le_public) mrel mrel'
 }.
 
 (* memory relation - equals *)
@@ -62,18 +81,37 @@ Record mrelT_propsT (t:Type) (ops:mrelT_opsT t): Prop := mkmrelT_propsT {
 Definition mrelT_ops_equals: mrelT_opsT unit :=
   mkmrelT_opsT
     (fun _ _ _ _ s1 s2 => state_mem s1 = state_mem s2)
-    (fun _ v1 v2 => Val.lessdef v1 v2)
+    (fun _ v1 v2 => v1 = v2)
     (fun _ _ => True)
     (fun _ _ => True).
 
-Program Definition mrelT_props_equals: mrelT_propsT mrelT_ops_equals := mkmrelT_propsT _ _ _ _ _ _.
+Lemma mrelT_ops_equals_equal_list mrel v1 v2:
+  v1 = v2 <-> list_forall2 (mrelT_ops_equals.(sem_value) mrel) v1 v2.
+Proof.
+  revert v2.
+  induction v1; intros; constructor; intro H; inv H; try constructor; simpl; auto.
+  - apply IHv1. auto.
+  - inv H2. f_equal. apply IHv1. auto.
+Qed.
+
+Program Definition mrelT_props_equals: mrelT_propsT mrelT_ops_equals := mkmrelT_propsT _ _ _ _ _ _ _.
 Next Obligation. repeat constructor. Qed.
 Next Obligation. repeat constructor. Qed.
-Next Obligation. inv H. auto. Qed.
 Next Obligation.
   exists tt. exists WF.elt. inv H1. inv H2. simpl.
   exploit program_lsim_init_mem_match; eauto. intro X.
   unfold fundef in *. rewrite H1 in X. inv X. auto.
+Qed.
+Next Obligation.
+  simpl in *. apply (mrelT_ops_equals_equal_list mrel args1 args2) in Hargs. subst. inv Hs0.
+  exists tt. exists WF.elt. eexists. eexists. eexists.
+  split; [eauto|]. split.
+  - constructor; eauto. eapply external_call_symbols_preserved; eauto.
+    + eapply symbols_preserved; eauto.
+    + intros. exploit varinfo_preserved; eauto. instantiate (1 := b).
+      unfold fundef. destruct (Genv.find_var_info (Genv.globalenv p1) b), (Genv.find_var_info (Genv.globalenv p2) b); intro X; inv X; auto.
+      f_equal. destruct g; auto.
+  - split; auto.
 Qed.
 
 (* memory relation - extends *)
@@ -85,7 +123,16 @@ Definition mrelT_ops_extends: mrelT_opsT unit :=
     (fun _ _ => True)
     (fun _ _ => True).
 
-Program Definition mrelT_props_extends: mrelT_propsT mrelT_ops_extends := mkmrelT_propsT _ _ _ _ _ _.
+Lemma mrelT_ops_extends_lessdef_list mrel v1 v2:
+  Val.lessdef_list v1 v2 <-> list_forall2 (mrelT_ops_extends.(sem_value) mrel) v1 v2.
+Proof.
+  revert v2.
+  induction v1; intros; constructor; intro H; inv H; constructor; auto.
+  - apply IHv1. auto.
+  - apply IHv1. auto.
+Qed.
+
+Program Definition mrelT_props_extends: mrelT_propsT mrelT_ops_extends := mkmrelT_propsT _ _ _ _ _ _ _.
 Next Obligation. repeat constructor. Qed.
 Next Obligation. repeat constructor. Qed.
 Next Obligation. inv H. auto. Qed.
@@ -95,14 +142,17 @@ Next Obligation.
   unfold fundef in *. rewrite H1 in X. inv X.
   apply Mem.extends_refl.
 Qed.
-
-Lemma mrelT_ops_extends_lessdef_list mrel v1 v2:
-  Val.lessdef_list v1 v2 <-> list_forall2 (mrelT_ops_extends.(sem_value) mrel) v1 v2.
-Proof.
-  revert v2.
-  induction v1; intros; constructor; intro H; inv H; constructor; auto.
-  - apply IHv1. auto.
-  - apply IHv1. auto.
+Next Obligation.
+  simpl in *. apply (mrelT_ops_extends_lessdef_list mrel args1 args2) in Hargs. inv Hs0.
+  exploit external_call_mem_extends; eauto. intros [vres_tgt [m2_tgt [Hef2 [Hvres [Hm2 _]]]]].
+  exists tt. exists WF.elt. eexists. eexists. eexists.
+  split; [eauto|]. split.
+  - constructor; eauto. eapply external_call_symbols_preserved; eauto.
+    + eapply symbols_preserved; eauto.
+    + intros. exploit varinfo_preserved; eauto. instantiate (1 := b).
+      unfold fundef. destruct (Genv.find_var_info (Genv.globalenv p1) b), (Genv.find_var_info (Genv.globalenv p2) b); intro X; inv X; auto.
+      f_equal. destruct g; auto.
+  - split; auto.
 Qed.
 
 Section LSIM.
